

$$X = \begin{pmatrix} 1 & -1 \\ 1 & 1 \\ 4 & 4 \\ 6 & 6 \end{pmatrix}$$

$$y = \begin{pmatrix} -1 \\ 2 \\ 3 \\ 4 \end{pmatrix}$$

$$\theta = (X^T X)^{-1} X^T y$$

$$= \left[\begin{pmatrix} 1 & 1 & 4 & 6 \\ -1 & 1 & 4 & 6 \end{pmatrix} \cdot \begin{pmatrix} 1 & -1 \\ 1 & 1 \\ 4 & 4 \\ 6 & 6 \end{pmatrix} \right]^{-1} X^T y$$

$$= \begin{pmatrix} 4 & 10 \\ 10 & 54 \end{pmatrix}^{-1} X^T y$$

$$= \frac{1}{216 - 100} \cdot \begin{pmatrix} 54 & -10 \\ -10 & 4 \end{pmatrix} X^T y$$

$$= \frac{1}{116} \cdot \begin{pmatrix} 54 & -10 \\ -10 & 4 \end{pmatrix} \begin{pmatrix} 1 & 1 & 4 & 6 \\ -1 & 1 & 4 & 6 \end{pmatrix} \cdot y$$

$$= \frac{1}{116} \cdot \begin{pmatrix} 64 & 44 & 14 & -6 \\ -14 & -6 & 6 & 14 \end{pmatrix} \cdot \begin{pmatrix} -1 \\ 2 \\ 3 \\ 4 \end{pmatrix}$$

$$= \frac{1}{116} \cdot \begin{pmatrix} 42 \\ 76 \end{pmatrix} \approx \begin{pmatrix} 0,362 \\ 0,65 \end{pmatrix}$$